theories/Util/Arith/FloatArith/Proofs.v
@@ -1,7 +1,7 @@
-From Coq Require Import Morphisms Lia Qround Sint63 Uint63 NArith PArith ZArith QArith Floats.
-From NeuralNetInterp.Util Require Import Default.
-From NeuralNetInterp.Util.Arith Require Import FloatArith.Definitions.
-From NeuralNetInterp.Util.Tactics Require Import DestructHead BreakMatch.
+From Coq Require Import Lqa Qabs Qround Morphisms Lia Qround Sint63 Uint63 NArith PArith ZArith QArith Floats.
+From NeuralNetInterp.Util Require Import Default SolveProperEqRel.
+From NeuralNetInterp.Util.Arith Require Import FloatArith.Definitions QArith.
+From NeuralNetInterp.Util.Tactics Require Import DestructHead BreakMatch UniquePose.
 Local Open Scope float_scope.
 #[local] Coercion Z.of_N : N >-> Z.
 #[local] Coercion inject_Z : Z >-> Q.
@@ -17,9 +17,9 @@ Module PrimFloat.
   #[local] Notation eta2 x := (fst x, snd x).
   Lemma fst_frshiftexp_spec : forall f, Prim2SF (fst (frshiftexp f)) = fst (SFfrexp prec emax (Prim2SF f)).
   Proof. intro f; generalize (frshiftexp_spec f); destruct frshiftexp; intros <-; reflexivity. Qed.
-  Lemma snd_frshiftexp_spec : forall f, to_Z (snd (frshiftexp f)) = (snd (SFfrexp prec emax (Prim2SF f)) + shift)%Z.
+  Lemma snd_frshiftexp_spec : forall f, Uint63.to_Z (snd (frshiftexp f)) = (snd (SFfrexp prec emax (Prim2SF f)) + shift)%Z.
   Proof. intro f; generalize (frshiftexp_spec f); destruct frshiftexp; intros <-; cbn [snd]; lia. Qed.
-  Lemma frshiftexp_spec_eta : forall f, let (m,e) := eta2 (frshiftexp f) in (Prim2SF m, ((to_Z e) - shift)%Z) = SFfrexp prec emax (Prim2SF f).
+  Lemma frshiftexp_spec_eta : forall f, let (m,e) := eta2 (frshiftexp f) in (Prim2SF m, ((Uint63.to_Z e) - shift)%Z) = SFfrexp prec emax (Prim2SF f).
   Proof. intro f; generalize (frshiftexp_spec f); destruct frshiftexp; intros <-; reflexivity. Qed.
 
   #[export] Hint Rewrite
@@ -48,61 +48,209 @@ Module PrimFloat.
 
     next_up_spec
     next_down_spec
-  : float_spec.
+    : float_spec.
   #[export] Hint Rewrite <-
     opp_spec
-    abs_spec
+      abs_spec
 
-    eqb_spec
-    ltb_spec
-    leb_spec
+      eqb_spec
+      ltb_spec
+      leb_spec
 
-    compare_spec
+      compare_spec
 
-    classify_spec
-    mul_spec
-    add_spec
-    sub_spec
-    div_spec
-    sqrt_spec
+      classify_spec
+      mul_spec
+      add_spec
+      sub_spec
+      div_spec
+      sqrt_spec
 
-    of_uint63_spec
-    normfr_mantissa_spec
+      of_uint63_spec
+      normfr_mantissa_spec
 
-    frshiftexp_spec_eta
-    ldshiftexp_spec
+      frshiftexp_spec_eta
+      ldshiftexp_spec
 
-    next_up_spec
-    next_down_spec
-  : float_spec_rev.
+      next_up_spec
+      next_down_spec
+    : float_spec_rev.
 
-  #[export] Instance of_Q_pos_Proper : Proper (Qeq ==> eq) of_Q_pos.
+  #[export] Instance Q2SF_Proper : Proper (Qeq ==> eq) Q2SF.
   Proof.
     intros x y H.
-    cbv [of_Q_pos].
-    rewrite !(Qred_complete _ _ H); reflexivity.
+    cbv [Q2SF]; rewrite H.
+    repeat match goal with
+           | [ H : ?x == ?y, H' : context[?x] |- _ ] => rewrite !H in H'; rewrite ?H' in *
+           | _ => break_innermost_match_step
+           | [ H : ?x == ?y |- context[?x] ] => rewrite H
+           | [ H : ?x == ?y |- _ ] => is_var x; clear x H
+           end.
+    all: reflexivity.
   Qed.
 
-  Lemma of_to_Q f {nan pinf ninf}
-    : of_Q (@to_Q nan pinf ninf f)
+
+  #[export] Instance of_Q_Proper : Proper (Qeq ==> eq) of_Q.
+  Proof. cbv [of_Q]; now intros ?? ->. Qed.
+
+  Local Ltac make_cases _ :=
+    lazymatch goal with
+    | [ |- (?P /\ ?Q) \/ _ ]
+      => let H := fresh in
+         assert (H : P \/ ~P) by lra;
+         destruct H as [H|H];
+         [ left; split; [ assumption | ]
+         | right; make_cases () ]
+    | _ => idtac
+    end.
+  Lemma Q2SF_classify q
+    : (q == 0 /\ Q2SF q = S754_zero false)
+      \/ ((((-1) / (2^(-(emin-1)))%Z) <= q < 0)%Q /\ Q2SF q = S754_zero true)
+      \/ ((q <= -(2^emax)%Z)%Q /\ Q2SF q = S754_infinity true)
+      \/ (((2^emax)%Z <= q)%Q /\ Q2SF q = S754_infinity false)
+      \/ ((-(2^emax)%Z < q < (2^emax)%Z)%Q /\ forall m e, Q2SF q = S754_finite (negb (Qle_bool 0 q)) m e).
+  Proof.
+    make_cases ().
+    { rewrite H; reflexivity. }
+    all: cbv [Q2SF]; rewrite ?Qabs_alt; break_innermost_match.
+    all: rewrite ?Qeq_bool_iff, ?Qle_bool_iff in *.
+    all: vm_compute emin in *.
+    all: vm_compute emax in *.
+    all: cbv [prec emax] in *.
+    all: repeat first [ progress destruct_head'_and
+                      | match goal with
+                        | [ H : (_ * _ == 0)%Q |- _ ] => apply Qmult_integral in H; destruct H
+                        | [ H : Qle_bool ?x ?y = false |- _ ]
+                          => pose proof (@Qle_bool_iff x y); rewrite H in *; clear H
+                        | [ H : Qeq_bool ?x ?y = false |- _ ] => apply Qeq_bool_neq in H
+                        | [ H : false = true <-> ?P |- _ ]
+                          => assert (~P) by (rewrite <- H; congruence); clear H
+                        | [ H : ~?x <= ?y |- _ ] => assert (y < x) by lra; clear H
+                        | [ H : inject_Z ?x == 0 |- _ ]
+                          => assert (x = 0)%Z by (now apply inject_Z_injective); clear H
+                        | [ H : (_^_ = 0)%Z |- _ ]
+                          => rewrite Z.pow_eq_0_iff in H
+                        | [ H : (Z.log2 ?x + _ - _ < 0)%Z |- _ ]
+                          => clear -H; pose proof (Z.log2_nonneg x); lia
+                        | [ H : Z.leb _ _ = true |- _ ] => rewrite Z.leb_le in H
+                        end
+                      | progress destruct_head'_or
+                      | lra
+                      | lia
+                      | reflexivity ].
+    lazymatch goal with
+    | [ H : ((-1)/inject_Z (2^?x) <= ?q)%Q |- _ ]
+      => move H at bottom; cbv [Qle Qopp Qdiv Qnum Qden inject_Z Qmult] in H;
+         let xv := (eval cbv in x) in
+         change x with xv in H;
+         change (Qinv ((2^xv) # 1)) with (1 # (Z.to_pos (2^xv))) in H;
+         cbv beta iota in H
+    end.
+  Admitted.
+
+  Lemma to_of_Q' q {nan pinf ninf nzero}
+    : @to_Q nan pinf ninf nzero (of_Q q)
+      == if (Qle_bool ((-1) / (2^(-(emin-1)))%Z) q) && negb (Qle_bool 0 q)
+         then nzero
+         else if Qle_bool q (-(2^emax)%Z)
+              then ninf
+              else if Qle_bool (2^emax)%Z q
+                   then pinf
+                   else q.
+  Proof.
+    cbv [to_Q to_Q_cps of_Q].
+    rewrite Prim2SF_SF2Prim.
+    pose proof (Q2SF_classify q); repeat (destruct_head'_or; destruct_head'_and).
+    all: generalize dependent (Q2SF q); intros; subst.
+    { match goal with
+      | [ H : q == _ |- _ ] => rewrite !H; cbv -["=="]; lra
+      end. }
+    all: cbv [andb negb]; break_innermost_match.
+    all: repeat match goal with
+           | [ H : Qle_bool _ _ = true |- _ ] => rewrite Qle_bool_iff in H
+           | [ H : Qeq_bool _ _ = true |- _ ] => rewrite Qeq_bool_iff in H
+           | [ H : Qle_bool ?x ?y = false |- _ ]
+             => pose proof (@Qle_bool_iff x y); rewrite H in *; clear H
+           | [ H : Qeq_bool ?x ?y = false |- _ ] => apply Qeq_bool_neq in H
+           | [ H : false = true <-> ?P |- _ ]
+             => assert (~P) by (rewrite <- H; congruence); clear H
+           | [ H : ~?x <= ?y |- _ ] => assert (y < x) by (clear -H; lra); clear H
+           end.
+    all: try lra.
+    all: repeat match goal with
+           | [ H : ?q <= ?x, H' : ?y <= ?q |- _ ]
+             => unique assert (y <= x) by lra
+           | [ H : ?q < ?x, H' : ?y <= ?q |- _ ]
+             => unique assert (y < x) by lra
+           end.
+    all: try match goal with
+           | [ H : _ |- _ ]
+             => exfalso; revert H; clear;
+                lazymatch goal with
+                | [ H : _ |- _ ] => fail
+                | _ => idtac
+                end;
+                vm_compute; congruence
+           | [ H : forall m e, _ = _ :> spec_float |- _ ]
+             => exfalso; clear -H; epose (H _ _); discriminate
+           end.
+    3: {
+    2: {
+    vm_compute in H2.
+    vm_compute in H1, H2; congruence.
+                assert (H : y < x) by lra;
+                vm_compute in H; specialize (H eq_refl); exfalso; now apply H
+           end.
+    match goal with
+    | [ H : ?q < ?x, H' : ?y <= ?q |- _ ]
+      => let H := fresh in
+         assert (H : y < x) by lra;
+         vm_compute in H; specialize (H eq_refl); exfalso; now apply H
+    end.
+    vm_compute in H0.
+    vm_compute Z.pow in *.
+
+
+    rewrite !H; cbv -["=="]; lra.
+    vm_compute negb.
+    rewrite Bool.andb_false_r.
+    vm_compute.
+    all: match goal with H : Q2SF q = _ |- _ =>
+    cbv [Q2SF andb negb]; break_innermost_match.
+    all: rewrite ?Qle_bool_iff in *.
+    all: rewrite ?Qabs_pos in * by assumption.
+    all: rewrite ?Qeq_bool_iff in *.
+
+    2: { assumption.
+        if is_nan f
+        then of_Q nan
+        else if is_infinity f
+             then if f <? 0 then of_Q ninf else of_Q pinf
+             else if is_zero f && get_sign f
+                  then of_Q nzero
+                  else f.
+
+  Lemma of_to_Q' f {nan pinf ninf nzero}
+    : of_Q (@to_Q nan pinf ninf nzero f)
       = if is_nan f
         then of_Q nan
         else if is_infinity f
              then if f <? 0 then of_Q ninf else of_Q pinf
-             else if is_zero f
-                  then abs f
+             else if is_zero f && get_sign f
+                  then of_Q nzero
                   else f.
   Proof.
     cbv [to_Q to_Q_cps is_infinity is_nan is_zero].
     pose proof (SF2Prim_Prim2SF f) as H.
     destruct (Prim2SF f) eqn:H'; subst.
-    { destruct_head'_bool; vm_compute; reflexivity. }
-    { destruct_head'_bool; cbv -[of_Q]; reflexivity. }
-    { cbv -[of_Q]; reflexivity. }
-    { repeat autorewrite with float_spec.
+    1-3: destruct_head'_bool; cbv -[of_Q]; reflexivity.
+    { cbv [get_sign is_zero zero].
+      repeat autorewrite with float_spec.
       rewrite !H'.
-      vm_compute Prim2SF.
+      vm_compute (Prim2SF 0).
+      vm_compute (Prim2SF ∞).
       cbv [SFabs SFeqb SFltb SFcompare].
+      autorewrite with float_spec.
       rewrite !Z.compare_refl.
       rewrite Pos.compare_cont_refl.
       cbv [CompOpp].
@@ -110,6 +258,7 @@ Module PrimFloat.
         [
         | let s := lazymatch goal with s : bool |- _ => s end in
           pose s as sv; destruct s; cbn [negb];
+          rewrite !H', ?Bool.andb_false_l;
           let sv := (eval cbv in sv) in
           set (s := sv); reflexivity ].
       apply Prim2SF_inj; rewrite H'.
